wip

theories/approxis/examples/prf.v
@@ -1,14 +1,21 @@
-From clutch.approxis Require Import approxis map list.
+From clutch.approxis Require Import approxis map list security_aux option.
 From clutch.approxis Require Export bounded_oracle.
 Set Default Proof Using "Type*".
 
-Section definition.
 
-  Variable Key Input Output : nat.
+(* rand_output is currently unused ; it would be useful if a PRF module had
+   abstract types. *)
+Class PRF :=
+  { card_key : nat
+  ; card_input : nat
+  ; card_output : nat
+  ; keygen : val
+  ; prf : val
+  ; rand_output : val
+  }.
 
-  Let keygen PRF_scheme : expr := Fst PRF_scheme.
-  Let prf PRF_scheme : expr := Fst (Snd PRF_scheme).
-  Let rand_output PRF_scheme : expr := Snd (Snd PRF_scheme).
+Section random_function.
+  Context `{PRF}.
 
   (* An idealised random function family. *)
   Definition random_function : val :=
@@ -19,14 +26,128 @@ Section definition.
         match: get "mapref" "x" with
         | SOME "y" => "y"
         | NONE =>
-            let: "y" := (rand #Output) in
+            let: "y" := (rand #card_output) in
             set "mapref" "x" "y";;
             "y"
         end.
 
-  Let q_calls := q_calls Input.
+  Definition lrel_key {Σ} : lrel Σ := lrel_int_bounded 0 card_key.
+  Definition lrel_input {Σ} : lrel Σ := lrel_int_bounded 0 card_input.
+  Definition lrel_output {Σ} : lrel Σ := lrel_int_bounded 0 card_output.
+  Definition lrel_keygen `{!approxisRGS Σ} : lrel Σ := (lrel_unit → lrel_key).
+  Definition lrel_prf `{!approxisRGS Σ} : lrel Σ := lrel_key → lrel_input → lrel_output.
 
-  Definition PRF : val :=
+  Definition lrel_PRF_Adv `{!approxisRGS Σ} := ((lrel_input → (lrel_option lrel_output)) → lrel_bool)%lrel.
+
+End random_function.
+
+
+Module LR_prf.
+  Import Ltac2.
+  Export LR_bounded.
+
+  Ltac2 Set pattern_of_lr2 as previous :=
+    fun lr (xs : constr list) =>
+      lazy_match! lr with
+      | lrel_input => bounded (get_head_name xs)
+      | lrel_output => bounded (get_head_name xs)
+      (* | lrel_message => bounded (get_head_name xs) *)
+      | lrel_key => bounded (get_head_name xs)
+      | _ => previous lr xs
+      end.
+
+  Ltac2 Set rel_vals as previous :=
+       fun lr =>
+         lazy_match! lr with
+         | (lrel_car lrel_output _ _) =>
+             ltac1:(iExists _ ; iPureIntro ; intuition lia)
+         | _ => previous lr
+         end.
+
+End LR_prf.
+Export LR_prf.
+
+Section random_function.
+  Context `{PRF}.
+
+  Fact random_function_sem_typed `{!approxisRGS Σ} A :
+    ⊢ REL random_function
+        << random_function : A → lrel_input → lrel_output.
+  Proof with (rel_pures_l ; rel_pures_r).
+    rel_arrow_val ; iIntros (??) "_".
+    rewrite /random_function...
+    rel_bind_r (init_map #()). iApply refines_init_map_r => /=... iIntros (map_r) "map_r".
+    rel_bind_l (init_map #()). iApply refines_init_map_l. iIntros (map_l) "map_l" => /=...
+    iApply (refines_na_alloc
+              ( ∃ (M : gmap nat val),
+                  map_list map_l M
+                  ∗ map_slist map_r M
+                  ∗ ⌜ ∀ y, y ∈ @map_img nat val (gmap nat val) _ (gset val) _ _ _ M
+                           → ∃ k : nat, y = #k ∧ k <= card_output ⌝
+                  ∗ ⌜ ∀ x, x ∈ elements (dom M) -> (x < S card_input)%nat ⌝
+              )%I
+              (nroot.@"RED")) ; iFrame.
+    iSplitL ; iFrame.
+    1: { iPureIntro; split ; [|set_solver].
+         intros y hy. exfalso. clear -hy.
+         rewrite map_img_empty in hy.
+         opose proof (proj1 (elem_of_empty y) hy). done.
+    }
+    iIntros "#Hinv".
+    rel_arrow_val. lrintro "x"...
+    iApply (refines_na_inv with "[$Hinv]"); [done|].
+    iIntros "(> (%M & map_l & map_r & %range_int & %dom_range) & Hclose)".
+    rel_bind_l (get _ _). rel_bind_r (get _ _).
+    opose proof (IZN x _) as [x' ->] => //. rename x' into x.
+    rel_apply_l (refines_get_l with "[-map_l] [$map_l]"). iIntros (?) "map_l #->"...
+    rel_apply_r (refines_get_r with "[-map_r] [$map_r]"). iIntros (?) "map_r #->"...
+
+    destruct (M !! x) as [y |] eqn:x_fresh ...
+    + iApply (refines_na_close with "[-]") ;
+        iFrame ; repeat iSplitL.
+      { iFrame. iNext. iFrame. iPureIntro. split. 2: set_solver. done. }
+      opose proof (elem_of_map_img_2 M x y x_fresh) as hy.
+      destruct (range_int y hy) as [y' [??]]. subst.
+      rel_vals.
+    + rel_apply (refines_couple_UU card_output id); first auto.
+      iIntros (y) "!> %"...
+      rel_apply_r (refines_set_r with "[-map_r] [$map_r]"). iIntros "map_r"...
+      rel_apply_l (refines_set_l with "[-map_l] [$map_l]"). iIntros "map_l"...
+      iApply (refines_na_close with "[-]") ;
+        iFrame ; repeat iSplitL. 1: iExists _ ; iFrame.
+      1: { iPureIntro.
+           repeat split ; last first.
+           - rewrite -Forall_forall.
+             rewrite dom_insert.
+             rewrite elements_union_singleton.
+             + apply Forall_cons_2. 1: lia. rewrite Forall_forall. done.
+             + apply not_elem_of_dom_2. done.
+           - intros y' hy'. rewrite (map_img_insert M x (#y)) in hy'.
+             rewrite elem_of_union in hy'. destruct hy'.
+             + exists y. set_solver.
+             + apply range_int.
+               opose proof (delete_subseteq M x).
+               eapply map_img_delete_subseteq. done.
+      }
+      rel_vals. Unshelve. all: apply _.
+  Qed.
+End random_function.
+
+(** PRF security definitions using the variant of q_calls with explicit bounds
+    checks in the code. **)
+Module bound_checks.
+
+  Context `{PRF}.
+
+  (* Variable Key Input Output : nat.
+
+     Let keygen PRF_scheme : expr := Fst PRF_scheme.
+     Let prf PRF_scheme : expr := Fst (Snd PRF_scheme).
+     Let rand_output PRF_scheme : expr := Snd (Snd PRF_scheme). *)
+
+  Let q_calls := q_calls card_input.
+
+  Definition PRF_real_rand : val :=
     λ:"b" "adv" "PRF_scheme" "Q",
       let: "key" := keygen "PRF_scheme" #() in
       let: "prf_key_b" :=
@@ -49,7 +170,7 @@ Section definition.
       let: "res" := ref list_nil in
       letrec: "loop" "i" :=
           if: "i" = #0 then #() else
-            let: "x" := rand #Input in
+            let: "x" := rand #card_input in
             let: "y" := "prf_key_b" "x" in
             "res" <- list_cons ("x", "y") (!"res") ;;
             "loop" ("i" - #1)
@@ -58,7 +179,7 @@ Section definition.
       ! "res".
 
   (* Rosulek, Def. 6.1 (PRF security) *)
-  (* NB: Rosulek samples the key from {0,1}^λ, we sample it from [0,Key]. *)
+  (* NB: Rosulek samples the key from {0,1}^λ, we sample it from [0,card_key]. *)
   Definition PRF_real : val :=
     λ:"PRF_scheme" "Q",
       let: "k" := keygen "PRF_scheme" #() in
@@ -83,7 +204,7 @@ Section definition.
         match: get hm "x" with
         | SOME "y" => "y"
         | NONE =>
-            let: "y" := (rand #Output) in
+            let: "y" := (rand #card_output) in
             set hm "x" "y";;
             "y"
         end.
@@ -92,7 +213,7 @@ Section definition.
         match: get "mapref" "x" with
         | SOME "y" => "y"
         | NONE =>
-            let: "y" := (rand #Output) in
+            let: "y" := (rand #card_output) in
             set "mapref" "x" "y";;
             "y"
         end.
@@ -174,4 +295,129 @@ Section definition.
     
   End spec_ideal.
 
-End definition.
+End bound_checks.
+
+(** PRF security definitions using the variant of q_calls using semantic typing
+    instead of bounds checks. **)
+Module sem.
+
+  Context `{PRF}.
+
+  Let q_calls := q_calls_poly.
+
+  Definition PRF_real : val :=
+    λ:"Q",
+      let: "k" := keygen #() in
+      let: "lookup" := prf "k" in
+      let: "oracle" := q_calls_poly #() #() "Q" "lookup" in
+      "oracle".
+
+  Definition PRF_rand : val :=
+    λ:"PRF_scheme" "Q",
+      let: "lookup" := random_function #() in
+      let: "oracle" := q_calls_poly #() #() "Q" "lookup" in
+      "oracle".
+
+  Section spec_ideal.
+
+    Context `{!approxisGS Σ}.
+
+    (* To hash a value v, we check whether it is in the map (i.e. it has been previously hashed).
+     If it has we return the saved hash value, otherwise we draw a hash value and save it in the map *)
+    Definition compute_rf_specialized hm : val :=
+      λ: "x",
+        match: get hm "x" with
+        | SOME "y" => "y"
+        | NONE =>
+            let: "y" := (rand #card_output) in
+            set hm "x" "y";;
+            "y"
+        end.
+    Definition compute_rf : val :=
+      λ: "mapref" "x",
+        match: get "mapref" "x" with
+        | SOME "y" => "y"
+        | NONE =>
+            let: "y" := (rand #card_output) in
+            set "mapref" "x" "y";;
+            "y"
+        end.
+
+    Definition is_random_function f m : iProp Σ :=
+      ∃ (mapref : loc), ⌜ f = compute_rf_specialized #mapref ⌝ ∗ map_list mapref ((λ b, LitV (LitInt b)) <$> m).
+
+    Definition is_srandom_function f m : iProp Σ :=
+      ∃ (mapref : loc), ⌜ f = compute_rf_specialized #mapref ⌝ ∗ map_slist mapref ((λ b, LitV (LitInt b)) <$> m).
+
+    #[global] Instance timeless_is_random_function f m :
+      Timeless (is_random_function f m).
+    Proof. apply _. Qed.
+
+    #[global] Instance timeless_is_srandom_function f m :
+      Timeless (is_srandom_function f m).
+    Proof. apply _. Qed.
+
+    Lemma wp_random_function E :
+      {{{ True }}}
+        random_function #() @ E
+        {{{ f, RET f; is_random_function f ∅ }}}.
+    Proof.
+      rewrite /random_function.
+      iIntros (Φ) "_ HΦ".
+      wp_pures.
+      wp_apply (wp_init_map with "[//]").
+      iIntros (?) "Hm". wp_pures.
+      iApply "HΦ". iExists _. rewrite fmap_empty. iFrame. eauto.
+    Qed.
+
+    Lemma spec_random_function E K:
+      ⤇ fill K (random_function #()) -∗
+      spec_update E (∃ (f:val), ⤇ fill K f ∗ is_srandom_function f ∅).
+    Proof.
+      rewrite /random_function.
+      iIntros "Hspec".
+      tp_pures.
+      tp_bind (init_map _).
+      iMod (spec_init_map with "[$]") as "(%&?&?)".
+      simpl. tp_pures.
+      iApply spec_update_ret.
+      by iFrame.
+    Qed.
+
+    Lemma wp_random_function_prev E f m (n : nat) (b : Z) :
+      m !! n = Some b →
+      {{{ is_random_function f m }}}
+        f #n @ E
+        {{{ RET #b; is_random_function f m }}}.
+    Proof.
+      iIntros (Hlookup Φ) "Hhash HΦ".
+      iDestruct "Hhash" as (hm ->) "H".
+      rewrite /compute_rf_specialized.
+      wp_pures.
+      wp_apply (wp_get with "[$]").
+      iIntros (vret) "(Hhash&->)".
+      rewrite lookup_fmap Hlookup /=. wp_pures. iModIntro. iApply "HΦ".
+      iExists _. eauto.
+    Qed.
+
+
+    Lemma spec_random_function_prev E f m (n : nat) (b : Z) K:
+      m !! n = Some b →
+      is_srandom_function f m -∗
+      ⤇ fill K (f #n) -∗
+      spec_update E (⤇ fill K #b ∗ is_srandom_function f m).
+    Proof.
+      iIntros (Hlookup) "Hhash Hspec".
+      iDestruct "Hhash" as (hm ->) "H".
+      rewrite /compute_rf_specialized.
+      tp_pures.
+      tp_bind (get _ _).
+      iMod (spec_get with "[$][$]") as "(?&?)".
+      simpl.
+      rewrite lookup_fmap Hlookup /=. tp_pures. iModIntro.
+      iFrame. auto.
+    Qed.
+
+  End spec_ideal.
+
+End sem.
