theories/approxis/examples/LR_tac.v
@@ -1,0 +1,104 @@
+From clutch.approxis Require Import approxis option.
+Set Default Proof Using "Type*".
+
+From Ltac2 Require Ltac2 Printf Option List.
+
+(* We define two extensible tactics for introducing and proving logical
+     relations. *)
+
+Import Ltac2 Printf Option List.
+
+Module Basic.
+  (* Importing LR_tac will provides a "batteries included" variant of the
+    tactics that deals with some of the syntactic built-in types. The bare
+    version ("without batteries") of the tactics can be accessed by importing
+    LR_tac.Basic. *)
+  Ltac2 mutable pattern_of_lr2 (lr : constr) (xs : constr list) : constr :=
+    lazy_match! lr with
+    | @lrel_unit _ => constr:("(->&->)")
+    | lrel_int =>
+        match xs with
+        | [] => '"(%&->&->)"
+        | x :: _ => let s := '(append "(%" ($x ++ "&->&->)")) in
+                    eval vm_compute in $s
+        end
+    | _ => Control.zero (Tactic_failure (Some (fprintf "no pattern found for lrel %t" lr)))
+    end.
+
+  Ltac2 mutable rel_vals (lr : constr) (* : unit *) :=
+    lazy_match! lr with
+    | @lrel_unit => eauto
+    | _ => Control.zero (Tactic_failure (Some (fprintf "Don't know how to solve lrel %t" lr)))
+    end.
+
+  Tactic Notation "lrintro" constr(x) :=
+    let f :=
+      ltac2val:
+        (lr xs |-
+           let pat := pattern_of_lr2
+                        (Option.get (Ltac1.to_constr lr))
+                        [(Option.get (Ltac1.to_constr xs))] in
+           Ltac1.of_constr pat) in
+    lazymatch goal with
+    | |- environments.envs_entails _ (lrel_car ?A _ _ -∗ _) =>
+        let x' := f A x in
+        iIntros x'
+    | |- environments.envs_entails _ (∀ (_ _ : val), lrel_car ?A _ _ -∗ _) =>
+        let x' := f A x in
+        iIntros (??) x'
+    end.
+
+  Tactic Notation "lrintro" := lrintro "".
+
+  Ltac rel_vals' :=
+    lazymatch goal with
+    (* | |- environments.envs_entails _ (_ (InjRV _) (InjRV _)) =>
+         iExists _,_ ; iRight ; iSplit ; [eauto|iSplit ; eauto]
+     | |- environments.envs_entails _ (_ (InjLV _) (InjLV _)) =>
+         iExists _,_ ; iLeft ; iSplit ; [eauto|iSplit ; eauto]
+     | |- environments.envs_entails _ (_ (_ , _)%V (_ , _)%V) =>
+         iExists _,_,_,_ ; iSplit ; [eauto|iSplit ; [eauto | iSplit]]
+     | |- environments.envs_entails _ (_ _ (lrel_int_bounded _ _) _ _) =>
+         iExists _ ; iPureIntro ; intuition lia
+     | |- environments.envs_entails _ (_ _ lrel_input _ _) =>
+         iExists _ ; iPureIntro ; intuition lia
+     | |- environments.envs_entails _ (_ _ lrel_output _ _) =>
+         iExists _ ; iPureIntro ; intuition lia *)
+    | |- environments.envs_entails _ ?lr =>
+        idtac "trying lr " lr ;
+        let f := ltac2:(lr |- rel_vals (Option.get (Ltac1.to_constr lr))) in
+        f lr
+    | _ => fail "rel_vals: case not covered"
+    end.
+  Ltac rel_vals := try (rel_values ; iModIntro) ; rel_vals'.
+
+End Basic.
+Export Basic.
+
+Ltac2 get_head_name xs := match xs with [] => '"" | x :: _ => x end.
+
+Module LR_option.
+
+  Ltac2 Set pattern_of_lr2 as previous :=
+    fun lr (xs : constr list) =>
+      lazy_match! lr with
+      | lrel_option ?a =>
+          let aa := previous a xs in
+          let u := previous 'lrel_unit xs in
+          let s := '(append "#(%" (" " ++ "&% &[(->&->&" ++ $u ++ ") | (->&->&"++$aa++")])")) in
+          eval vm_compute in $s
+      | _ => previous lr xs
+      end.
+
+  Ltac2 Set rel_vals as previous :=
+    fun lr =>
+      lazy_match! lr with
+      | (lrel_car _ (InjRV _) (InjRV _)) =>
+          ltac1:(iExists _,_ ; iRight ; iSplit ; [eauto | iSplit ; eauto])
+      | (lrel_car _ (InjLV _) (InjLV _)) =>
+          ltac1:(iExists _,_ ; iLeft ; iSplit ; [eauto | iSplit ; eauto])
+      | _ => previous lr
+      end.
+
+End LR_option.
+Export LR_option.
