theories/approxis/examples/bounded_oracle.v
@@ -1,6 +1,6 @@
 From clutch.prob_lang.typing Require Import tychk.
 From clutch.approxis Require Import approxis map list.
-From clutch.approxis.examples Require Import security_aux.
+From clutch.approxis.examples Require Import security_aux option.
 Set Default Proof Using "Type*".
 
 
